geometry/lean/Geometry/Basic.lean
@@ -32,6 +32,26 @@ structure Cell where
   y : Int
   deriving Repr, Inhabited, DecidableEq, BEq, Hashable
 
+theorem cell_beq_def (a b : Cell) : (a == b) = (a.x == b.x && a.y == b.y) := rfl
+
+instance : LawfulBEq Cell where
+  eq_of_beq {a b} h := by
+    rw [cell_beq_def] at h
+    have h1 : (a.x == b.x) = true := by
+      revert h
+      cases a.x == b.x <;> simp
+    have h2 : (a.y == b.y) = true := by
+      revert h
+      cases a.x == b.x <;> cases a.y == b.y <;> simp
+    have hx : a.x = b.x := eq_of_beq h1
+    have hy : a.y = b.y := eq_of_beq h2
+    cases a; cases b
+    simp only at hx hy
+    rw [hx, hy]
+  rfl {a} := by
+    rw [cell_beq_def]
+    simp
+
 /--
 Converts a Float to an Int by taking the floor and casting.
 -/
